Fix Source/CS.v -- (introduce one admit)

Source/CS.v
@@ -165,18 +165,18 @@ Inductive kstep (G: global_env) : state -> trace event -> state -> Prop :=
     imported_procedure (genv_interface G) C C' P  ->
     (* retrieve the procedure code *)
     find_procedure (genv_procedures G) C' P = Some P_expr ->
-    kstep G [State C, s, mem, Kcall C' P k, E_val (Int v), old_call_arg]
+    kstep G [State C, s, mem, Kcall C' P k, E_val v, old_call_arg]
             [:: ECall C P v C']
-            [State C', Frame C old_call_arg k :: s, mem, Kstop, P_expr, Int v]
+            [State C', Frame C old_call_arg k :: s, mem, Kstop, P_expr, v]
 | KS_InternalReturn: forall C s mem k v arg C' old_call_arg,
     C = C' ->
     kstep G [State C, Frame C' old_call_arg k :: s, mem, Kstop, E_val (Int v), arg] E0
             [State C', s, mem, k, E_val (Int v), old_call_arg]
 | KS_ExternalReturn: forall C s mem k v arg C' old_call_arg,
     C <> C' ->
-    kstep G [State C, Frame C' old_call_arg k :: s, mem, Kstop, E_val (Int v), arg]
+    kstep G [State C, Frame C' old_call_arg k :: s, mem, Kstop, E_val v, arg]
             [:: ERet C v C']
-            [State C', s, mem, k, E_val (Int v), old_call_arg].
+            [State C', s, mem, k, E_val v, old_call_arg].
 
 Lemma kstep_component G s t s' :
   kstep G s t s' ->
@@ -271,26 +271,26 @@ Definition eval_kstep (G : global_env) (st : state) : option (trace event * stat
       | _ => None
       end
     | Kcall C' P k' =>
-      match v with
-      | Int i =>
+      (*match v with
+      | Int i =>*)
         if C == C' then
           (* retrieve the procedure code *)
           do P_expr <- find_procedure (genv_procedures G) C' P;
-          ret (E0, [State C', Frame C arg k' :: s, mem, Kstop, P_expr, Int i])
+          ret (E0, [State C', Frame C arg k' :: s, mem, Kstop, P_expr, v])
         else if imported_procedure_b (genv_interface G) C C' P then
           (* retrieve the procedure code *)
           do P_expr <- find_procedure (genv_procedures G) C' P;
-          ret ([ECall C P i C'], [State C', Frame C arg k' :: s, mem, Kstop, P_expr, Int i])
+          ret ([ECall C P v C'], [State C', Frame C arg k' :: s, mem, Kstop, P_expr, v])
         else
           None
-      | _ => None
-      end
+      (*| _ => None
+      end*)
     | Kstop =>
-      match v, s with
-      | Int i, Frame C' old_call_arg k' :: s' =>
-        let t := if C == C' then E0 else [:: ERet C i C'] in
-        ret (t, [State C', s', mem, k', E_val (Int i), old_call_arg])
-      | _, _ => None
+      match (*v,*) s with
+      | (*Int i,*) Frame C' old_call_arg k' :: s' =>
+        let t := if C == C' then E0 else [:: ERet C v C'] in
+        ret (t, [State C', s', mem, k', E_val v, old_call_arg])
+      | (*_,*) _ => None
       end
     end
   | _ => None
@@ -354,7 +354,7 @@ Proof.
            reflexivity)
   end.
   - repeat simplify_option.
-    + case: (_ =P _) => [->|?]; econstructor; eauto.
+    + admit. (*case: (_ =P _) => [->|?]; econstructor; eauto.*)
     + econstructor; eauto.
     + econstructor; eauto.
     + econstructor; eauto.
@@ -364,10 +364,10 @@ Proof.
     + by econstructor; eauto; apply/eqP.
     + econstructor; eauto.
     + by econstructor; eauto; apply/eqP.
-    + econstructor; eauto; exact/eqP.
+    + admit. (*econstructor; eauto; exact/eqP.*)
     + econstructor; eauto; first exact/eqP/negbT.
       apply imported_procedure_iff. assumption.
-Qed.
+Admitted.
 
 Theorem eval_kstep_correct:
   forall G st t st',
@@ -394,14 +394,16 @@ Section Semantics.
 
   Lemma receptiveness_step:
     forall s t1 s1 t2,
-      kstep G s t1 s1 -> match_traces t1 t2 ->
+      kstep G s t1 s1 -> equal_and_nil_or_singleton t1 t2 ->
       exists s2, kstep G s t2 s2.
   Proof.
     intros s t1 s1 t2.
     intros Hkstep Hmatch_traces.
     inversion Hkstep; subst;
     inversion Hmatch_traces; subst;
-      try (eexists; apply Hkstep).
+      try (eexists; apply Hkstep);
+      match goal with H: event_equal _ _ |- _ => apply event_equal_equal in H end;
+      subst; eexists; exact Hkstep.
   Qed.
 
   Lemma singleton_traces:
